skip_list/spec/new.v
@@ -1,0 +1,100 @@
+From iris.algebra Require Import auth frac_auth gset.
+From iris.heap_lang Require Import proofmode.
+
+From SkipList.lib Require Import lock misc.
+From SkipList.skip_list Require Import inv node_rep code key_equiv.
+
+
+Local Open Scope Z.
+Module NewSpec (Params: SKIP_LIST_PARAMS).
+  Import Params.
+  Module Invariant := SkipListInv Params.
+  Import Invariant.
+
+  Section Proofs.
+    Context `{!heapGS Σ, !gset_list_unionGS Σ, lockG Σ} (N : namespace).
+
+    Theorem newLoop_spec (head: node_rep) (lvl: Z) (L: list (list node_rep)):
+      {{{ 
+        skip_list_equiv head lvl (nil :: L) ∅ ∅ 
+      }}}
+        newLoop (rep_to_node head) #lvl
+      {{{ h top_head L', RET #h;
+        h ↦ rep_to_node top_head
+        ∗
+        skip_list_equiv top_head MAX_HEIGHT L' ∅ ∅ 
+      }}}.
+    Proof.
+      iIntros (Φ) "Hlist HΦ".
+      iRevert (head lvl L) "Hlist HΦ".
+      iLöb as "IH".
+      iIntros (head lvl L) "Hlist HΦ".
+
+      wp_lam. wp_let. wp_alloc h as "Hh".
+      wp_pures. case_bool_decide; wp_if.
+      + iApply "HΦ". iModIntro.
+        assert (lvl = MAX_HEIGHT) as <- by congruence.
+        iFrame.
+      + wp_alloc t as "Ht". wp_let.
+        iDestruct "Ht" as "(Ht1 & Ht2)".
+        wp_apply (newlock_spec (node_inv t) with "[Ht1]").
+        { iExists tail; iFrame. }
+        iIntros (l) "#Hlock". iDestruct "Hlock" as (γ) "Hlock".
+        wp_pures.
+        set (top_head := (INT_MIN, Some t, Some h, l)).
+        rewrite (fold_rep_to_node top_head).
+
+        iApply ("IH" $! top_head (lvl+1) (nil :: L) with "[Hlist Hh Ht2]").
+        - iExists ∅, h, head.
+          assert (lvl + 1 - 1 = lvl) as -> by lia.
+          iFrame. 
+          iSplit; first done. iSplit; first done. iSplit; last done.
+          iExists nil. iSplit; first done. iSplit.
+          {
+            assert (node_lt top_head tail); last (simpl; auto).
+            rewrite /node_lt/node_key//=; apply HMIN_MAX.
+          }
+          iExists t, γ. by iFrame "# ∗".
+        - iNext; iApply "HΦ".
+    Qed.
+
+    Theorem new_spec : 
+      {{{ True }}}
+        new #()
+      {{{ v, RET v;
+        is_skip_list N v ∅
+      }}}.
+    Proof.
+      iIntros (Φ) "_ HΦ".
+      wp_lam. wp_alloc t as "Ht". wp_let.
+      iDestruct "Ht" as "(Ht1 & Ht2)".
+      wp_apply (newlock_spec (node_inv t) with "[Ht1]").
+      { iExists tail; iFrame. }
+      iIntros (l) "#Hlock". iDestruct "Hlock" as (γ) "Hlock".
+      wp_pures.
+      rewrite (fold_rep_to_node (INT_MIN, Some t, None, l)).
+      set (bot_head := (INT_MIN, Some t, None, l)).
+
+      wp_apply (newLoop_spec _ _ nil with "[Ht2]").
+      { 
+        iSplit; first done. iSplit; first done. iSplit; last done.
+        iExists nil. iSplit; first done. iSplit.
+        { 
+          assert (node_lt bot_head tail); last (simpl; auto).
+          rewrite /node_lt/node_key//=; apply HMIN_MAX.
+        }
+        iExists t, γ. by iFrame "# ∗".
+      }
+
+      iIntros (h top_head L) "[Hh Hlist]"; wp_pures.
+      iMod (inv_alloc N ⊤ (skip_list_inv top_head ∅) 
+        with "[Hlist Hlock]") as "#Hinv".
+      { iNext; iExists ∅, L. by iFrame "# ∗". }
+      iModIntro; iApply "HΦ". 
+      iExists h, top_head, ∅.
+      iSplit; first rewrite /key_equiv //.
+      by iFrame "# ∗".
+    Qed.
+
+  End Proofs.
+End NewSpec.
